trying to lower simple negotiation functions with Tahina

src/tls/Negotiation.Version.fst
@@ -7,29 +7,28 @@ open TLSConstants // for leqPV and the configuration
 open FStar.Error
 open TLSError
 
-// updated excerpts of Negotiation re: protocol versions
+#reset-options "--query_stats --using_facts_from '* -FStar.Reflection -FStar.Tactics -EverCrypt -Crypto -Spec -Hacl'" 
 
 /// ---- PROTOCOL VERSIONS ----
 ///
 /// The protocol version is negotiated in ClientHello and ServerHello,
-/// using two overlapping mechanisms.  We currently implement only TLS
-/// 1.2 and 1.3, and the negotiated version can be further constrained
-/// in the connection initial configuration.
+/// using two overlapping mechanisms for TLS_1p3 and earlier versions.  
 
-// 19-01-04 TODO? 
+// 19-01-04 possible code improvements: 
 // * replace min/max_version in config with the payload of the supported_version extension.
-// * refine TLSConstants.protocolVersion with implemented instead of not Unknown. 
+// * refine TLSConstants.protocolVersion with implemented instead of not Unknown (this re-binding is confusing) 
 
-let implemented pv =
-  pv = TLS_1p2 || pv = TLS_1p3
+/// We currently implement only TLS 1.2 and 1.3, and the negotiated
+/// version can be further constrained in the connection initial
+/// configuration.
 
-let (<=) = leqPV
+let implemented pv = pv = TLS_1p2 || pv = TLS_1p3
 
 let supported cfg pv =
   implemented pv &&
-  cfg.min_version <= pv && pv <= cfg.max_version
+  cfg.min_version `leqPV` pv && pv `leqPV` cfg.max_version
 
-// negotiation failures; unnecessary?
+// negotiation failures; does that help with extraction or verification?
 // private let illegal       #a msg: result a = fatal #a Illegal_parameter msg
 // private let unsupported   #a msg: result a = fatal #a Unsupported_extension msg
 // private let fatal_version #a msg: result a = fatal #a Protocol_version msg
@@ -40,8 +39,8 @@ let supported cfg pv =
 /// configuration. We may provide more flexible configurations by replacing
 /// min/max_version with a list of supported versions.
 
-#push-options "--query_stats --z3rlimit 100" // 19-01-04 too slow? note the refinement on the length of the inner lists. 
-(*
+(* 
+// an earlier variant, presumaly harder to lower and extract.
 let offer_versions cfg: option clientHelloExtension =
   match cfg.min_version, cfg.max_version with
   | TLS_1p3, TLS_1p3 -> Some (CHE_supported_versions [TLS_1p3])
@@ -50,45 +49,102 @@ let offer_versions cfg: option clientHelloExtension =
   | _                -> None
 *)
 
-// Alternative code, easier to refine and extract; worth the trouble? 
-private let cons_supported cfg pv pvs = if supported cfg pv then pv::pvs else pvs 
+// an auxiliary function; its first version was simpler, but led to timeouts below.
+// let snoc_supportedVersion cfg pv pvs = 
+//   if supported cfg pv then pvs @ [pv] else pvs 
+
+// its tedious elaboration--complicating our spec
+let snoc_supportedVersion
+  (cfg:config) 
+  (pv:Parsers.ProtocolVersion.protocolVersion) 
+  (pvs:list Parsers.ProtocolVersion.protocolVersion): 
+  (pvs1:list Parsers.ProtocolVersion.protocolVersion {List.length pvs1 <= List.length pvs + 1}) 
+= 
+  if supported cfg pv then (
+    List.lemma_snoc_length (pvs,pv);
+    pvs @ [pv] ) 
+  else pvs 
+
+// 19-01-26 slow TC, due to constructor refinements? 
+#push-options "--z3rlimit 100"
 let support cfg: result clientHelloExtension =
-  let vs = cons_supported cfg TLS_1p2 [] in 
-  let vs = cons_supported cfg TLS_1p3 vs in 
+  let vs = snoc_supportedVersion cfg TLS_1p3 [] in 
+  let vs = snoc_supportedVersion cfg TLS_1p2 vs in 
   if List.isEmpty vs 
   then fatal Internal_error "configuration must include a supported protocol version"
   else Correct (CHE_supported_versions vs)
-#pop-options
+#pop-options 
 
-(* too large?
-let same_supported cfg: Lemma (supported_versions cfg == supported_versions2 cfg) =
-  match cfg.min_version, cfg.max_version with
-  | SSL_3p0, SSL_3p0 -> assert_norm (supported_versions cfg == supported_versions2 cfg)
-  | SSL_3p0, TLS_1p0 -> assert_norm (supported_versions cfg == supported_versions2 cfg)
-  | SSL_3p0, TLS_1p1 -> assert_norm (supported_versions cfg == supported_versions2 cfg)
-  | SSL_3p0, TLS_1p2 -> assert_norm (supported_versions cfg == supported_versions2 cfg)
-  | SSL_3p0, TLS_1p3 -> assert_norm (supported_versions cfg == supported_versions2 cfg)
-  | TLS_1p0, SSL_3p0 -> assert_norm (supported_versions cfg == supported_versions2 cfg)
-  | TLS_1p0, TLS_1p0 -> assert_norm (supported_versions cfg == supported_versions2 cfg)
-  | TLS_1p0, TLS_1p1 -> assert_norm (supported_versions cfg == supported_versions2 cfg)
-  | TLS_1p0, TLS_1p2 -> assert_norm (supported_versions cfg == supported_versions2 cfg)
-  | TLS_1p0, TLS_1p3 -> assert_norm (supported_versions cfg == supported_versions2 cfg)
-  | TLS_1p1, SSL_3p0 -> assert_norm (supported_versions cfg == supported_versions2 cfg)
-  | TLS_1p1, TLS_1p0 -> assert_norm (supported_versions cfg == supported_versions2 cfg)
-  | TLS_1p1, TLS_1p1 -> assert_norm (supported_versions cfg == supported_versions2 cfg)
-  | TLS_1p1, TLS_1p2 -> assert_norm (supported_versions cfg == supported_versions2 cfg)
-  | TLS_1p1, TLS_1p3 -> assert_norm (supported_versions cfg == supported_versions2 cfg)
-  | TLS_1p2, SSL_3p0 -> assert_norm (supported_versions cfg == supported_versions2 cfg)
-  | TLS_1p2, TLS_1p0 -> assert_norm (supported_versions cfg == supported_versions2 cfg)
-  | TLS_1p2, TLS_1p1 -> assert_norm (supported_versions cfg == supported_versions2 cfg)
-  | TLS_1p2, TLS_1p2 -> assert_norm (supported_versions cfg == supported_versions2 cfg)
-  | TLS_1p2, TLS_1p3 -> assert_norm (supported_versions cfg == supported_versions2 cfg)
-  | TLS_1p3, SSL_3p0 -> assert_norm (supported_versions cfg == supported_versions2 cfg)
-  | TLS_1p3, TLS_1p0 -> assert_norm (supported_versions cfg == supported_versions2 cfg)
-  | TLS_1p3, TLS_1p1 -> assert_norm (supported_versions cfg == supported_versions2 cfg)
-  | TLS_1p3, TLS_1p2 -> assert_norm (supported_versions cfg == supported_versions2 cfg)
-  | TLS_1p3, TLS_1p3 -> assert_norm (supported_versions cfg == supported_versions2 cfg)
-*)
+open FStar.Integers 
+open LowParse.Low.Base 
+open Mem
+
+// migrate to LowParse? 
+let live_slice_pos h0 out p0 = live_slice h0 out /\ p0 <= out.len 
+
+#push-options "--z3rlimit 100" 
+val write_supportedVersions
+  (cfg:config) 
+  (out:slice) (p0:UInt32.t) : Stack (result UInt32.t) 
+  (requires fun h0 -> live_slice_pos h0 out p0) 
+  (ensures fun h0 r h1 -> 
+    LowStar.Modifies.(modifies (loc_slice_from out p0) h0 h1) /\ (
+    match r with 
+    | Error z -> True
+    | Correct p1 -> 
+      match support cfg with 
+      | Error _ -> False 
+      | Correct che -> valid_content_pos clientHelloExtension_parser h1 out p0 che p1 ))
+#pop-options 
+
+val write_supportedVersion 
+  (cfg: config) 
+  (pv: Parsers.ProtocolVersion.protocolVersion) 
+  (out: slice) (pl p0: UInt32.t) : Stack UInt32.t
+  (requires fun h0 -> 
+    valid_list protocolVersion_parser h0 out pl p0 /\
+    v p0 + 2 <= v out.len
+    //19-01-26 slower & causing a timeout below: [v out.len - v p0 >= 2]
+    //19-01-26 much slower: [out.len - p0 >= 2ul]
+    )
+  (ensures fun h0 p1 h1 -> 
+    valid_list protocolVersion_parser h1 out pl p1 /\
+    v p1 - v p0 <= 2 /\ 
+    LowStar.Buffer.modifies (loc_slice_from_to out p0 p1) h0 h1 /\
+    contents_list protocolVersion_parser h1 out pl p1 == snoc_supportedVersion cfg pv (contents_list protocolVersion_parser h0 out pl p0))
+
+#push-options "--z3rlimit 100"
+let write_supportedVersion cfg pv out pl p0 =
+  if supported cfg pv then (
+    let p1 = protocolVersion_writer pv out p0 in
+    let h1 = get () in
+    valid_list_snoc protocolVersion_parser h1 out pl p0;
+    p1
+  ) else p0
+
+let write_supportedVersions cfg out p0 = 
+  if out.len - p0 < 10ul then fatal Internal_error "output buffer" else 
+  let pvl = p0 + 2ul in // extension tag
+  let pl0 = pvl + 1ul in // length of the list of ciphersuites. 
+  let h = get () in
+  valid_list_nil protocolVersion_parser h out pl0; 
+  let pl = write_supportedVersion cfg TLS_1p3 out pl0 pl0 in 
+  let pl = write_supportedVersion cfg TLS_1p2 out pl0 pl in
+  if pl = pl0 then fatal Internal_error "configuration must include a supported protocol version" else 
+    let h = get () in
+    valid_list_cons_recip protocolVersion_parser h out pl0 pl; 
+    Extensions.finalize_supportedVersions out pvl pl;
+    let h = get () in
+
+    //19-01-26 stuck here.
+    // assume(valid clientHelloExtension_CHE_supported_versions_parser h out pvl);
+    assume False;
+    Extensions.finalize_clientHelloExtension_supported_versions out p0;
+    Correct pl
+// this kind of code is hard to get right, as the programmer needs to
+// know every detail of the wire format, including its byte offsets
+// and explicit proof steps---every error takes 10' 
+
 
 /// (2) Server chooses a supported version
 ///
@@ -98,20 +154,19 @@ let same_supported cfg: Lemma (supported_versions cfg == supported_versions2 cfg
 
 // temporary; will use Parsers.ClientHello.clientHello 
 type ch = HandshakeMessages.ch
-private let offered_version o = o.HandshakeMessages.ch_protocol_version 
-private let offered_extensions o = o.HandshakeMessages.ch_extensions 
+let offered_version o = o.HandshakeMessages.ch_protocol_version 
+let offered_extensions o = o.HandshakeMessages.ch_extensions 
 
-// We ignore the "minimal protocol version" signalled in the packet
-// header; this is fine since our server never accepts any proposal
-// below the "maximal protocol version".
+/// We ignore the "minimal protocol version" signalled in the packet
+/// header; this is fine since our server never accepts any proposal
+/// below the "maximal protocol version".
 
 private let correct #a (x:a): result a = Correct x
- 
-#set-options "--z3rlimit 100"
+
 val choose: cfg:config -> ch -> result (pv:protocolVersion{ supported cfg pv })
 let choose cfg ch =
   let legacy_max_pv = offered_version ch in // offer.Parsers.ClientHello.version in
-  if TLS_1p3 <= legacy_max_pv then
+  if TLS_1p3 `leqPV` legacy_max_pv then
     fatal Protocol_version "protocol version negotiation: bad legacy proposal"
   else
     match List.Tot.find CHE_supported_versions? (offered_extensions ch) with
@@ -127,7 +182,52 @@ let choose cfg ch =
       match List.Helpers.find_aux cfg supported vs with
       | Some v -> correct v
       | None -> fatal Protocol_version "protocol version negotiation: mismatch"
-#reset-options
+
+(*
+// 19-01-26 TODO lowering this function requires two iterators on the
+// received sequence of client-supported extensions. (Not sure how to
+// write them parametrically, since they need to be parameterized by
+// accessors, readers, and jumpers.) Use supportedVersions_nth instead?  
+
+let rec find_supportedVersions parser jumper reader filter input p pmax =
+  if p = pmax then None else 
+    let v = reader input p in 
+    if filter v then Some v else
+      let p = jumper parser input p in 
+      find_supportedVersions parser jumper reader filter input p max  
+
+val choose_low:
+  cfg:config -> 
+  input:slice -> pch:UInt32.t -> Stack (result protocolVersion) 
+  (requires fun h0 -> 
+    valid Parsers.ClientHello.clientHello_parser h0 input pch) 
+  (ensures fun h0 r h1 -> r = 
+    let ch = contents Parsers.ClientHello.clientHello_parser h0 input p in 
+    LowStar.Modifies.(modifies loc_none h0 h1) /\ 
+    r == choose cfg ch)
+
+let choose_low cfg input pch = 
+  let ppv = accessor_clientHello_version input pch in 
+  let legacy_max_pv = protocolVersion_reader input ppv in 
+  if TLS_1p3 `leqPV` legacy_max_pv then
+    fatal Protocol_version "protocol version negotiation: bad legacy proposal"
+  else
+    let pches = accessor_clientHello_extensions input in 
+    match LowParse.find_list CHE_supported_versions? input pches with
+    | None ->
+      // legacy negotiation: we pick at most TLS 1p2
+      if legacy_max_pv = TLS_1p2 && supported cfg TLS_1p2 then
+        correct TLS_1p2
+      else
+        fatal Protocol_version "protocol version negotiation: mismatch"
+
+    | Some (p_supported_versions) ->
+      // new extension-based negotiation: we pick the first client offer supported by the server
+      match LowParse.find_list_aux cfg supported input p_supported_versions with
+      | Some v -> correct v
+      | None -> fatal Protocol_version "protocol version negotiation: mismatch"  
+*)
+
 
 /// (3) Client validates the server's choice
 
@@ -145,8 +245,8 @@ let isSentinelRandomValue client_pv server_pv server_random =
   let open FStar.Bytes in
   let down = bytes_of_string "DOWNGRD" in
   assume(length down = 7 /\ length (abyte 1z) = 1 /\ length (abyte 0z) = 1); //18-12-16 TODO how?
-  (server_pv <= TLS_1p2 && TLS_1p3 <= client_pv && server_random = down @| abyte 1z) ||
-  (server_pv <= TLS_1p1 && TLS_1p2 <= client_pv && server_random = down @| abyte 0z)
+  (server_pv `leqPV` TLS_1p2 && TLS_1p3 `leqPV` client_pv && server_random = down @| abyte 1z) ||
+  (server_pv `leqPV` TLS_1p1 && TLS_1p2 `leqPV` client_pv && server_random = down @| abyte 0z)
 
 val accept:
   cfg: config ->
@@ -167,7 +267,7 @@ let accept cfg pv ses sr =
       match List.Tot.find SHE_supported_versions? ses with
       | None -> pv // old style
       | Some (SHE_supported_versions pv) -> pv in
-    if TLS_1p3 <= chosen && pv <> TLS_1p2 then
+    if TLS_1p3 `leqPV` chosen && pv <> TLS_1p2 then
       fatal Illegal_parameter "extension-based version negotiation requires TLS 1.2 apparent version"
     else
     if isSentinelRandomValue cfg.max_version chosen sr then 
